src/Spec/Hoare.v
@@ -11,7 +11,7 @@ behavior. *)
 Record SpecProps T R State :=
   { pre: Prop;
     post: State -> T -> Prop;
-    recovered: State -> R -> Prop; }.
+    alternate: State -> R -> Prop; }.
 
 Definition Specification A T R State := A -> State -> SpecProps T R State.
 
@@ -20,10 +20,10 @@ Definition spec_exec A T R State (spec: Specification A T R State) :
   fun s s' r => forall a,
     (spec a s).(pre) -> (spec a s).(post) s' r.
 
-Definition spec_rexec A T R State (spec: Specification A T R State) :
+Definition spec_aexec A T R State (spec: Specification A T R State) :
   relation State State R :=
   fun s s' r => forall a,
-    (spec a s).(pre) -> (spec a s).(recovered) s' r.
+    (spec a s).(pre) -> (spec a s).(alternate) s' r.
 
 Definition spec_impl A A'
            `(spec1: Specification A' T R State)
@@ -32,8 +32,8 @@ Definition spec_impl A A'
          exists a', (spec1 a' s).(pre) /\
                (forall s' v, (spec1 a' s).(post) s' v ->
                         (spec2 a s).(post) s' v) /\
-               (forall s' rv, (spec1 a' s).(recovered) s' rv ->
-                         (spec2 a s).(recovered) s' rv).
+               (forall s' rv, (spec1 a' s).(alternate) s' rv ->
+                         (spec2 a s).(alternate) s' rv).
 
 Definition op_spec `(sem: Dynamics Op State) `(op : Op T) : Specification unit T unit State :=
   fun (_:unit) state =>
@@ -41,7 +41,7 @@ Definition op_spec `(sem: Dynamics Op State) `(op : Op T) : Specification unit T
       pre := True;
       post :=
         fun state' v => sem.(step) op state state' v;
-      recovered :=
+      alternate :=
         fun state' r =>
           r = tt /\ (state' = state \/ exists v, sem.(step) op state state' v);
     |}.
@@ -51,95 +51,183 @@ Section Hoare.
   Context `(sem: Dynamics Op State).
   Notation proc := (proc Op).
   Notation exec := sem.(exec).
+  Notation exec_crash := sem.(exec_crash).
   Notation rexec := sem.(rexec).
 
-  Definition proc_ok A T R
+  Definition proc_rspec A T R
              (p: proc T) (rec: proc R)
              (spec: Specification A T R State) :=
     exec p ---> spec_exec spec /\
-    rexec p rec ---> spec_rexec spec.
+    rexec p rec ---> spec_aexec spec.
 
-  Theorem proc_ok_expand A T R
+  Definition proc_cspec A T
+             (p: proc T)
+             (spec: Specification A T unit State) :=
+    exec p ---> spec_exec spec /\
+    exec_crash p ---> spec_aexec spec.
+
+  Theorem proc_rspec_expand A T R
           (p: proc T) (rec: proc R)
           (spec: Specification A T R State) :
-    proc_ok p rec spec <->
+    proc_rspec p rec spec <->
     forall a s,
       (spec a s).(pre) ->
       (forall s' v, exec p s s' v ->
                (spec a s).(post) s' v) /\
       (forall s' rv, rexec p rec s s' rv ->
-                (spec a s).(recovered) s' rv).
+                (spec a s).(alternate) s' rv).
   Proof.
-    unfold proc_ok, rimpl, spec_exec, spec_rexec; split; intros.
+    unfold proc_rspec, rimpl, spec_exec, spec_aexec; split; intros.
     - intuition eauto 10.
     - split; intros.
       specialize (H a x); intuition eauto.
       specialize (H a x); intuition eauto.
   Qed.
 
-  Theorem spec_impl_relations A A'
+  Theorem proc_cspec_expand A T (p: proc T)
+          (spec: Specification A T unit State) :
+    proc_cspec p spec <->
+    forall a s,
+      (spec a s).(pre) ->
+      (forall s' v, exec p s s' v ->
+               (spec a s).(post) s' v) /\
+      (forall s' rv, exec_crash p s s' rv ->
+                (spec a s).(alternate) s' rv).
+  Proof.
+    unfold proc_cspec, rimpl, spec_exec, spec_aexec; split; intros.
+    - intuition eauto 10.
+    - split; intros.
+      specialize (H a x); intuition eauto.
+      specialize (H a x); intuition eauto.
+  Qed.
+
+  Theorem proc_rspec_impl A A'
           `(spec1: Specification A' T R State)
           `(spec2: Specification A T R State)
           p rec :
     spec_impl spec1 spec2 ->
-    proc_ok p rec spec1 ->
-    proc_ok p rec spec2.
+    proc_rspec p rec spec1 ->
+    proc_rspec p rec spec2.
   Proof.
     unfold spec_impl; intros.
-    pose proof (proj1 (proc_ok_expand _ _ _) H0); clear H0.
-    apply proc_ok_expand; intros.
+    pose proof (proj1 (proc_rspec_expand _ _ _) H0); clear H0.
+    apply proc_rspec_expand; intros.
     specialize (H a s); propositional.
     specialize (H1 a' s); propositional.
     eauto 10.
   Qed.
 
-  Theorem proc_ok_exec_equiv A T `(spec: Specification A T R State)
+  Theorem proc_cspec_impl A A'
+          `(spec1: Specification A' T unit State)
+          `(spec2: Specification A T unit State)
+          p :
+    spec_impl spec1 spec2 ->
+    proc_cspec p spec1 ->
+    proc_cspec p spec2.
+  Proof.
+    unfold spec_impl; intros.
+    pose proof (proj1 (proc_cspec_expand _ _) H0); clear H0.
+    apply proc_cspec_expand; intros.
+    specialize (H a s); propositional.
+    specialize (H1 a' s); propositional.
+    eauto 10.
+  Qed.
+
+  Theorem proc_rspec_exec_equiv A T `(spec: Specification A T R State)
           (p p': proc T) `(rec: proc R):
       exec_equiv sem p p' ->
-      proc_ok p' rec spec ->
-      proc_ok p rec spec.
-  Proof. unfold proc_ok. intros ->; auto. Qed.
+      proc_rspec p' rec spec ->
+      proc_rspec p rec spec.
+  Proof. unfold proc_rspec. intros ->; auto. Qed.
 
-  Theorem proc_ok_rx A T A' T' R `(spec: Specification A T R State)
+  Theorem proc_cspec_exec_equiv A T `(spec: Specification A T unit State)
+          (p p': proc T):
+      exec_equiv sem p p' ->
+      proc_cspec p' spec ->
+      proc_cspec p spec.
+  Proof. unfold proc_cspec. intros ->; auto. Qed.
+
+  Theorem proc_rspec_rx A T A' T' R `(spec: Specification A T R State)
                            `(p: proc T) `(rec: proc R)
                            `(rx: T -> proc T')
                            `(spec': Specification A' T' R State):
-      proc_ok p rec spec ->
+      proc_rspec p rec spec ->
       (forall a' state, pre (spec' a' state) ->
                exists a, pre (spec a state) /\
                     (forall r,
-                        proc_ok (rx r) rec
+                        proc_rspec (rx r) rec
                           (fun (_:unit) state' =>
                              {| pre := post (spec a state) state' r;
                                 post :=
                                   fun (state'' : State) r =>
                                     post (spec' a' state) state'' r;
-                                recovered :=
+                                alternate :=
                                   fun (state'' : State) r =>
-                                    recovered (spec' a' state) state'' r |})
+                                    alternate (spec' a' state) state'' r |})
                     ) /\
-                    (forall (r: R) (state': State), recovered (spec a state) state' r ->
-                             recovered (spec' a' state) state' r)) ->
-      proc_ok (Bind p rx) rec spec'.
+                    (forall (r: R) (state': State), alternate (spec a state) state' r ->
+                             alternate (spec' a' state) state' r)) ->
+      proc_rspec (Bind p rx) rec spec'.
   Proof.
-    unfold proc_ok at 3. intros (Hp_ok&Hp_rec) Hrx.
+    unfold proc_rspec at 3. intros (Hp_ok&Hp_rec) Hrx.
     split.
     - simpl; rew Hp_ok.
       intros state state' t' (t&(state_mid&Hspec_mid&Hexec_mid)) a' Hpre'.
       specialize (Hrx _ _ Hpre') as (a&Hpre&Hok&Hrec).
-      specialize (Hok t). rewrite proc_ok_expand in Hok.
+      specialize (Hok t). rewrite proc_rspec_expand in Hok.
       destruct (Hok tt state_mid) as (Hrx_ok&Hrx_rec); simpl; eauto.
     - rewrite rexec_unfold. rewrite rexec_unfold in Hp_rec.
       simpl. rewrite exec_crash_idem, bind_dist_r.
       apply rel_or_elim.
       + rewrite Hp_rec; auto.
-        intros state state' r Hspec_rexec a' Hpre'.
+        intros state state' r Hspec_aexec a' Hpre'.
         specialize (Hrx _ _ Hpre') as (a&Hpre&?&Hrec); eauto.
       + rewrite bind_assoc, Hp_ok.
         intros state state' t' (t&(state_mid&Hspec_mid&Hcrash_mid)) a' Hpre'.
       specialize (Hrx _ _ Hpre') as (a&Hpre&Hok&Hrec).
-      specialize (Hok t). rewrite proc_ok_expand in Hok.
+      specialize (Hok t). rewrite proc_rspec_expand in Hok.
       destruct (Hok tt state_mid) as (Hrx_ok&Hrx_rec); simpl; eauto.
+  Qed.
+
+  Theorem proc_cspec_rx A T A' T' `(spec: Specification A T unit State)
+                           `(p: proc T)
+                           `(rx: T -> proc T')
+                           `(spec': Specification A' T' unit State):
+      proc_cspec p spec ->
+      (forall a' state, pre (spec' a' state) ->
+               exists a, pre (spec a state) /\
+                    (forall r,
+                        proc_cspec (rx r)
+                          (fun (_:unit) state' =>
+                             {| pre := post (spec a state) state' r;
+                                post :=
+                                  fun (state'' : State) r =>
+                                    post (spec' a' state) state'' r;
+                                alternate :=
+                                  fun (state'' : State) r =>
+                                    alternate (spec' a' state) state'' r |})
+                    ) /\
+                    (forall (r:  unit) (state': State), alternate (spec a state) state' r ->
+                             alternate (spec' a' state) state' r)) ->
+      proc_cspec (Bind p rx) spec'.
+  Proof.
+    unfold proc_cspec at 3. intros (Hp_ok&Hp_rec) Hrx.
+    split.
+    - simpl; rew Hp_ok.
+      intros state state' t' (t&(state_mid&Hspec_mid&Hexec_mid)) a' Hpre'.
+      specialize (Hrx _ _ Hpre') as (a&Hpre&Hok&Hrec).
+      specialize (Hok t). rewrite proc_cspec_expand in Hok.
+      destruct (Hok tt state_mid) as (Hrx_ok&Hrx_rec); simpl; eauto.
+    - simpl. rewrite exec_crash_idem.
+      apply rel_or_elim.
+      + rewrite Hp_rec; auto.
+        intros state state' r Hspec_aexec a' Hpre'.
+        specialize (Hrx _ _ Hpre') as (a&Hpre&?&Hrec); eauto.
+      + rewrite Hp_ok.
+        intros state state' t' (t&(state_mid&Hspec_mid&Hcrash_mid)) a' Hpre'.
+        specialize (Hrx _ _ Hpre') as (a&Hpre&Hok&Hrec).
+        specialize (Hok t). rewrite proc_cspec_expand in Hok.
+        destruct (Hok tt state_mid) as (Hrx_ok&Hrx_rec); simpl; eauto.
   Qed.
 
   (** ** Reasoning about the [Ret] return operation.
@@ -162,19 +250,16 @@ Section Hoare.
 
   Definition rec_noop `(rec: proc R) (wipe: State -> State -> Prop) :=
     forall T (v:T),
-      proc_ok
+      proc_rspec
         (Ret v) rec
         (fun (_:unit) state =>
            {| pre := True;
               post := fun state' r => r = v /\
                                       state' = state;
-              recovered := fun state' _ => wipe state state'; |}).
+              alternate := fun state' _ => wipe state state'; |}).
 
-  Definition proc_loopspec A `(rec': proc unit) `(rec: proc unit)
-             `(spec: Specification A unit unit State):=
-    (pure tt + rexec rec' rec);; exec rec' ---> spec_exec spec.
 
-  (** A more general theorem about specifications for [Ret], which
+  (** A more general theorem about recovery specifications for [Ret], which
     we will use as part of our proof automation, says
     that [Ret v] meets a specification [spec] if the [rec_noop]
     theorem holds (i.e., the recovery procedure is correctly
@@ -182,45 +267,58 @@ Section Hoare.
     [spec] matches the [wipe] relation:
    *)
 
-  Theorem ret_spec A T R (wipe: State -> State -> Prop) `(spec: Specification A T R State)
+  Theorem ret_rspec A T R (wipe: State -> State -> Prop) `(spec: Specification A T R State)
           (v:T) (rec: proc R):
     rec_noop rec wipe ->
     (forall a state, pre (spec a state) ->
                      post (spec a state) state v /\
                      forall state', wipe state state' ->
-                                    forall (r : R), recovered (spec a state) state' r) ->
-    proc_ok (Ret v) rec spec .
+                                    forall (r : R), alternate (spec a state) state' r) ->
+    proc_rspec (Ret v) rec spec .
   Proof.
-    unfold proc_ok; intros Hnoop Himpl; split.
+    unfold proc_rspec; intros Hnoop Himpl; split.
     - intros state state' t Hexec a Hpre.
       inversion Hexec; subst. specialize (Himpl _ _ Hpre). intuition.
     - destruct (Hnoop _ v) as (?&->).
-      unfold spec_rexec.
+      unfold spec_aexec.
       intros s s' r Hl a Hpre. specialize (Hl tt).
       eapply Himpl; eauto.
       eapply Hl; simpl; eauto.
   Qed.
 
+  Theorem ret_cspec A T `(spec: Specification A T unit State)
+          (v:T):
+    (forall a state, pre (spec a state) ->
+                     post (spec a state) state v /\
+                     alternate (spec a state) state tt) ->
+    proc_cspec (Ret v) spec .
+  Proof.
+    unfold proc_cspec; intros Himpl; split;
+    intros state state' t Hexec a Hpre;
+    inversion Hexec; subst; specialize (Himpl _ _ Hpre); intuition.
+  Qed.
+
   (** Define what it means for a spec to be idempotent: *)
-  Definition idempotent A T `(spec: Specification A T unit State) :=
+  Definition idempotent A T R `(spec: Specification A T R State) :=
     forall a state,
       pre (spec a state) ->
-      forall v state', recovered (spec a state) state' v ->
-              (** idempotency: recovered condition implies precondition to
+      forall v state', alternate (spec a state) state' v ->
+              (** idempotency: alternate condition implies precondition to
                  re-run on every crash *)
               exists a', pre (spec a' state') /\
                     (** postcondition transitivity: establishing the
-                       postcondition from a recovered state is sufficient to
+                       postcondition from a alternate state is sufficient to
                        establish it with respect to the original initial
                        state (note all with the same ghost state) *)
                     forall rv state'', post (spec a' state') state'' rv ->
                                   post (spec a state) state'' rv.
 
 
+  (*
   (* Idempotents theorem: *)
   Theorem idempotent_loopspec A `(rec: proc unit) `(rec': proc unit)
         `(spec: Specification A unit unit State)
-        (Hspec: proc_ok rec' rec spec):
+        (Hspec: proc_rspec rec' rec spec):
         idempotent spec ->
         proc_loopspec rec' rec spec.
   Proof.
@@ -235,12 +333,14 @@ Section Hoare.
       specialize (Hrs' a Hpre). unfold idempotent in H.
       edestruct H as (a'&Hpre'&Hpost); eauto.
   Qed.
+   *)
 
+  (*
   Theorem compose_recovery A A' A'' `(spec: Specification A'' T unit State)
                                `(rspec: Specification A' unit unit State)
                                `(spec': Specification A T unit State)
                                `(p: proc T) `(rec: proc unit) `(rec': proc unit)
-        (Hspec: proc_ok p rec spec)
+        (Hspec: proc_rspec p rec spec)
         (Hrspec: proc_loopspec rec' rec rspec)
         (Hspec_spec':
            forall (a:A) state, pre (spec' a state) ->
@@ -248,14 +348,14 @@ Section Hoare.
                         pre (spec a'' state) /\
                         (forall v state', post (spec a'' state) v state' ->
                                  post (spec' a state) v state') /\
-                        (forall v state', recovered (spec a'' state) state' v ->
+                        (forall v state', alternate (spec a'' state) state' v ->
                                  exists a', pre (rspec a' state') /\
                                        forall v' state'',
                                          post (rspec a' state') state'' v' ->
-                                         recovered (spec' a state) state'' v')):
-        proc_ok p (Bind rec (fun _ => rec')) spec'.
+                                         alternate (spec' a state) state'' v')):
+        proc_rspec p (Bind rec (fun _ => rec')) spec'.
   Proof.
-    unfold proc_ok; intros; split.
+    unfold proc_rspec; intros; split.
     - destruct Hspec as (->&?).
       intros s s' t Hspec a Hpre.
       edestruct Hspec_spec' as (a''&?&Hp&?); eauto.
@@ -272,7 +372,7 @@ Section Hoare.
               _ <- exec rec;
               exec rec'
                    --->
-                   spec_rexec spec').
+                   spec_aexec spec').
       { rew <- seq_star_none in Hrec.
         rew <- rel_or_introl in Hrspec.
         rew Hrspec.
@@ -285,27 +385,7 @@ Section Hoare.
         destruct H2 as (?&?). eapply H3. eapply Hexec_rspec. eauto.
       }
   Abort.
-
-  Theorem op_spec_correct T (op: Op T) rec (* (wipe: State -> State -> Prop) *):
-    rec_noop rec eq ->
-    proc_ok (Prim op) rec (op_spec sem op).
-  Proof.
-    unfold proc_ok; intros Hnoop; split.
-    - intros state state' t Hexec a Hpre; eauto.
-    - unfold rexec, spec_rexec.
-      simpl. rewrite bind_dist_r. apply rel_or_elim.
-      * destruct (Hnoop _ tt) as (?&->).
-        intros s s' [] Hl a Hpre. specialize (Hl tt).
-        split; eauto. intuition.
-      * rewrite bind_assoc.
-        destruct (Hnoop _ tt) as (?&Hr).
-        setoid_rewrite Hr.
-        unfold spec_rexec.
-        intros s s' [] Hl a Hpre.
-        inversion Hl as (?&?&?&Hrest). specialize (Hrest tt I). split; eauto.
-        right.  eexists; eauto. simpl in Hrest. subst. eauto.
-  Qed.
-
+   *)
 
   (** In some situations, the precondition of a specification
     may define variables or facts that you want to [intros].
@@ -316,25 +396,77 @@ Section Hoare.
     arbitrary Prop in question as a hypothesis about [state0].
   *)
 
-  Theorem spec_intros A T R `(spec: Specification A T R State)
+  Theorem rspec_intros A T R `(spec: Specification A T R State)
           `(p: proc T) `(rec: proc R):
       (forall a state0,
           pre (spec a state0) ->
-          proc_ok p rec
+          proc_rspec p rec
             (fun (_:unit) state =>
                {| pre := state = state0;
                   post :=
                     fun state' r => post (spec a state) state' r;
-                  recovered :=
-                    fun state' r => recovered (spec a state) state' r;
+                  alternate :=
+                    fun state' r => alternate (spec a state) state' r;
                |})) ->
-      proc_ok p rec spec.
+      proc_rspec p rec spec.
   Proof.
-    unfold proc_ok at 2; intros H.
+    unfold proc_rspec at 2; intros H.
     split; intros s s' r Hexec a Hpre; eapply H; simpl; eauto using tt.
   Qed.
 
+  Theorem cspec_intros A T `(spec: Specification A T unit State)
+          `(p: proc T):
+      (forall a state0,
+          pre (spec a state0) ->
+          proc_cspec p
+            (fun (_:unit) state =>
+               {| pre := state = state0;
+                  post :=
+                    fun state' r => post (spec a state) state' r;
+                  alternate :=
+                    fun state' r => alternate (spec a state) state' r;
+               |})) ->
+      proc_cspec p spec.
+  Proof.
+    unfold proc_cspec at 2; intros H.
+    split; intros s s' r Hexec a Hpre; eapply H; simpl; eauto using tt.
+  Qed.
+
+  (*
+  Theorem op_spec_correct T (op: Op T) rec (* (wipe: State -> State -> Prop) *):
+    rec_noop rec eq ->
+    proc_rspec (Prim op) rec (op_spec sem op).
+  Proof.
+    unfold proc_rspec; intros Hnoop; split.
+    - intros state state' t Hexec a Hpre; eauto.
+    - unfold rexec, spec_aexec.
+      simpl. rewrite bind_dist_r. apply rel_or_elim.
+      * destruct (Hnoop _ tt) as (?&->).
+        intros s s' [] Hl a Hpre. specialize (Hl tt).
+        split; eauto. intuition.
+      * rewrite bind_assoc.
+        destruct (Hnoop _ tt) as (?&Hr).
+        setoid_rewrite Hr.
+        unfold spec_aexec.
+        intros s s' [] Hl a Hpre.
+        inversion Hl as (?&?&?&Hrest). specialize (Hrest tt I). split; eauto.
+        right.  eexists; eauto. simpl in Hrest. subst. eauto.
+  Qed.
+   *)
+
+  Theorem op_spec_correct T (op: Op T):
+    proc_cspec (Prim op) (op_spec sem op).
+  Proof.
+    unfold proc_cspec; split.
+    - intros state state' t Hexec a Hpre; eauto.
+    - simpl. apply rel_or_elim.
+      * intros s s' [] Hl a Hpre. simpl. split; auto.
+        firstorder.
+      * intros s s' [] Hl a Hpre.
+        inversion Hl as (?&?&?&Hrest). inversion Hrest; subst.
+        firstorder.
+  Qed.
 
 End Hoare.
 
-Ltac spec_intros := intros; eapply spec_intros; intros.
+Ltac spec_intros := intros; first [ eapply rspec_intros | eapply cspec_intros ] ; intros.
